

ST 661 Note

Frances Lin

1/20/2022

Outline

- Idempotent matrix
- Matrix calculus

Last time

Let A_1 be the 1st subspace and A_2 be the second subspace, then we can write x s.t.

$$x = A_1x + A_2x \quad \forall x \in \mathbb{R}^n$$

$$I = A_1 + A_2, \quad \text{rank}(I) = 2$$
$$\text{rank}(A_1) = 1, \quad \text{rank}(A_2) = 2$$

Both A_1 and A_2 are idempotent matrices.

Now, we pick $x \in \mathbb{R}^3$ and decompose it s.t.

$$x = A_1x + A_2x,$$

where

$$\text{rank}(A_1) = 2 \quad \text{a plane}, \quad \text{rank}(A_2) = 1 \quad \text{a line},$$

so

$$\text{rank}(I) = 3 = 2 + 1 = \text{rank}(A_1) + \text{rank}(A_2).$$

Thm

$I : nxn$, $I = A_1 + A_2 + \dots A_k$ (k can be anything $\leq n$), where each A_i is nxn symmetric of rank r_i .

If $\sum_{i=1}^k r_i = n$ (no gain or loss of rank), then

- A_i (each A_i) is idempotent $i = 1, 2, \dots k$
- $A_i A_j = 0$ $i \neq j$ (complementary)

Comment. In general, $\text{rank}(A + B) \neq \text{rank}(A) + \text{rank}(B)$. So when it is equal, then all A_i are idempotent.

e.g. $n = 2$

$$I = \begin{bmatrix} 1 & 0 \\ 0 & 1 \end{bmatrix} = \begin{bmatrix} 1 & 0 \\ 0 & 0 \end{bmatrix} + \begin{bmatrix} 0 & 0 \\ 0 & 1 \end{bmatrix} = A_1 + A_2$$

So, $\text{rank}(A_1) + \text{rank}(A_2) = 2 = \text{rank}(I)$.

\Rightarrow

- i) A_1, A_2 are both idempotent
- ii) $A_1 A_2 = 0$ Info does not overlap.

$$x = \begin{bmatrix} x_1 \\ x_2 \end{bmatrix}$$

$$A_1 x = \begin{bmatrix} 1 & 0 \\ 0 & 0 \end{bmatrix} \begin{bmatrix} x_1 \\ x_2 \end{bmatrix},$$

projecting to x axis.

$$A_2 x = \begin{bmatrix} 0 & 0 \\ 0 & 1 \end{bmatrix} \begin{bmatrix} x_1 \\ x_2 \end{bmatrix},$$

projecting to y axis.

e.g.

$$I = \begin{bmatrix} 1 & 0 \\ 0 & 1 \end{bmatrix} = \begin{bmatrix} \frac{1}{2} & 0 \\ 0 & \frac{1}{2} \end{bmatrix} + \begin{bmatrix} \frac{1}{2} & 0 \\ 0 & \frac{1}{2} \end{bmatrix}$$

In this case,

$$\text{rank}(I) = 2 \neq 2 + 2 = \text{rank}(A_1) + \text{rank}(A_2)$$

Condition is not met. Info overlap.

ii)

$$A_1 A_2 = \begin{bmatrix} \frac{1}{4} & 0 \\ 0 & \frac{1}{4} \end{bmatrix} \neq 0,$$

so info overlap.

Vector or matrix calculus (derivatives mostly)

1. vector \rightarrow scalar

$u = f(x)$, where u is a scalar, x is a column vector and

$$x = \begin{bmatrix} x_1 & x_2 & \cdots & x_p \end{bmatrix}^T = \begin{bmatrix} x_1 \\ x_2 \\ \vdots \\ x_p \end{bmatrix},$$

then

$$\frac{\partial u}{\partial x} = \begin{bmatrix} \frac{\partial u}{\partial x_1} \\ \frac{\partial u}{\partial x_2} \\ \vdots \\ \frac{\partial u}{\partial x_p} \end{bmatrix}.$$

Thm

Let $u = a^T x$ and $a = (a_1, a_2, \dots, a_p)^T$ is a constant vector, then

$$\frac{\partial u}{\partial x} = a,$$

i.e.

$$\frac{\partial u}{\partial x_1} = a_1.$$

Thm

$u = X^T A X$ (quadratic form). A is symmetric matrix of constants.

$$u = X^T A X = \sum_{i=1}^n \sum_{j=1}^n a_{ij} x_i x_j,$$

then

$$\frac{\partial u}{\partial x} = \frac{\partial X^T A X}{\partial x} = 2AX,$$

which is analogous to taking

$$\frac{\partial}{\partial x}(ax^2) = 2ax.$$

Proof.

$$\frac{\partial u}{\partial x_i} = \frac{\partial X^T A X}{\partial x_i} = \dots \quad \square$$

2. matrix \rightarrow scalar

$\mu = f(X)$ X is a $p \times p$ square matrix. e.g.

$$\frac{\partial u}{\partial X} = \begin{bmatrix} \frac{\partial u}{\partial x_{11}} & \frac{\partial u}{\partial x_{12}} & \dots & \frac{\partial u}{\partial x_{1p}} \\ \vdots & & & \\ \frac{\partial u}{\partial x_{p1}} & \dots & \dots & \frac{\partial u}{\partial x_{pp}} \end{bmatrix}.$$

Notation. x is vector. X is matrix.

Thm

$u = \text{tr}(XA)$ where A is a $p \times p$ constant matrix (This is more general than $u = \text{tr}(X)$), then

$$\frac{\partial u}{\partial X} = \frac{\partial}{\partial X} \text{tr}(XA)$$

$$= A + A^T - \text{diag}(A).$$

Proof.

$$\text{tr}(XA) = \sum_{i=1}^p \sum_{j=1}^p x_{ij} a_{ji}$$

Verify the above.

$$\frac{\partial}{\partial x_{ij}} = \begin{cases} a_{ij} + a_{ji} & i \neq j \\ a_{ii} & i = j \end{cases}$$

The idea is that $\text{tr}()$ is a linear function.

Thm

$u = \log(\det(X))$, X is $p \times p$ p.d., then

$$\frac{\partial}{\partial X}(\det(X)) = 2X^{-1} - \text{diag}(X^{-1}).$$

Proof. Skip here.

E.g. log likelihood of MVN's sigma term.

3. scalar \rightarrow vector or matrix

$A : A(x)$ where x is scalar.

$A : (a_{ij})$ is matrix.

Properties

$A = A(x)$ and $B = B(x)$

i) If A and B have the same dim, then

$$\frac{\partial}{\partial X}(A + B) = \frac{\partial A}{\partial X} + \frac{\partial B}{\partial X}.$$

ii) If A and B are conformal for multiplication, then

$$\frac{\partial}{\partial X}(AB) = \frac{\partial A}{\partial X}B + A\frac{\partial B}{\partial X}$$

$$\frac{\partial}{\partial X}(ABC) = \frac{\partial A}{\partial X}BC + A\frac{\partial B}{\partial X}C + AB\frac{\partial C}{\partial X}.$$

Thm

$A = A(x)$ is nonsingular, $A^{-1} = A^{-1}(x)$ is another matrix function of x , then

$$\frac{\partial}{\partial X}A^{-1} = -A^{-1} + \frac{\partial A}{\partial X}A^{-1}$$

Proof. Start with $AA^{-1} = I$. $\frac{\partial A}{\partial X}$, A^{-1} , and A are known, then

$$0 = \frac{\partial AA^{-1}}{\partial X} = \frac{\partial A}{\partial X}A^{-1} + A\frac{\partial A^{-1}}{\partial X},$$

so

$$A\frac{\partial A^{-1}}{\partial X} = -\frac{\partial A}{\partial X}A^{-1}$$

$$\frac{\partial A^{-1}}{\partial X} = -A^{-1}\frac{\partial A}{\partial X}A^{-1} \quad \square$$

Thm

$A = A(x)$ Now A is indexed by scalar. A is $n \times n$, symmetric, p.d. $\log(\det(A))$ is a scalar function of x , then

$$\frac{\partial}{\partial X} \log(\det(A)) = \text{tr}(A^{-1} \frac{\partial A}{\partial X})$$

Proof. $A = CDC^T$

First, show that

$$\begin{aligned} \frac{\partial}{\partial X} \log(\det(D)) &= \frac{\partial}{\partial X} \log(\lambda_1, \dots, \lambda_n) = \frac{\partial}{\partial X} (\log(\lambda_1), \dots, \log(\lambda_n)) = \sum_{i=1}^n \frac{1}{\lambda_i} \frac{\partial \lambda_i}{\partial X} \\ &= \text{tr}(D^{-1} \frac{\partial D}{\partial X}) \\ &= \text{tr} \left(\begin{bmatrix} \frac{1}{\lambda_1} & 0 & 0 \\ 0 & \ddots & 0 \\ 0 & 0 & \frac{1}{\lambda_n} \end{bmatrix} \begin{bmatrix} \frac{\partial \lambda_1}{\partial X} & 0 & 0 \\ 0 & \ddots & 0 \\ 0 & 0 & \frac{\partial \lambda_n}{\partial X} \end{bmatrix} \right) \\ &= \text{tr} \left(\begin{bmatrix} \frac{1}{\lambda_1} \frac{\partial \lambda_1}{\partial X} & 0 & 0 \\ 0 & \ddots & 0 \\ 0 & 0 & \frac{1}{\lambda_n} \frac{\partial \lambda_n}{\partial X} \end{bmatrix} \right) \\ &= \sum_{i=1}^n \frac{1}{\lambda_i} \frac{\partial \lambda_i}{\partial X}. \end{aligned}$$

Next, for general A , we want to diagonalize it: $A = CDC^T$.

Recall that $\det(CDC^T) = \det(D)$ since $C \dots$, so

$$\frac{\partial}{\partial X} \log(\det(A)) = \frac{\partial}{\partial X} \log(\det(D)) = \text{tr}(D^{-1} \frac{\partial D}{\partial X}) = \text{tr}(A^{-1} \frac{\partial A}{\partial X})$$

? remains to be shown.

Start with RHS, we have that

$$\begin{aligned} \text{tr}(A^{-1} \frac{\partial A}{\partial X}) &= \text{tr}((CDC^T)^{-1} \frac{\partial(CDC^T)}{\partial X}) \\ &= \text{tr}((CD^{-1}C^T)((\frac{\partial C}{\partial X})DC^T + C(\frac{\partial D}{\partial X})C^T) + CD(\frac{\partial C^T}{\partial X})) \\ &= \text{tr}(CD^{-1}C^T(\frac{\partial C}{\partial X})DC^T) + \text{tr}(CD^{-1}C^T C(\frac{\partial D}{\partial X})C^T) + \text{tr}(CD^{-1}C^T CD(\frac{\partial C^T}{\partial X})) \end{aligned}$$

Recall that $\text{tr}(AB) = \text{tr}(BA)$

$$= \text{tr}(D^{-1}C^T \frac{\partial C}{\partial X} DI) + \dots + \dots = \text{tr}(C^T \frac{\partial C}{\partial X}) + \text{tr}(D^{-1} \frac{\partial D}{\partial X}) + \text{tr}(C \frac{\partial C^T}{\partial X})$$

To show that

$$\text{tr}(A^{-1} \frac{\partial A}{\partial X}) = \text{tr}(D^{-1} \frac{\partial D}{\partial X}),$$

need to show

$$\text{tr}(C^T \frac{\partial C}{\partial X}) + \text{tr}(C \frac{\partial C^T}{\partial X}) = 0$$

$$\text{tr}(C^T \frac{\partial C}{\partial X}) + \text{tr}(C \frac{\partial C^T}{\partial X}) = \text{tr}(C^T \frac{\partial C}{\partial X} + C \frac{\partial C^T}{\partial X}),$$

but this is not quite the same.

However, notice that

$$\frac{\partial I}{\partial X} = \frac{\partial(CC^T)}{\partial X} = \frac{\partial C}{\partial X} C^T + C \frac{\partial C^T}{\partial X} = 0,$$

since I does not depend on X .

Reverse the order of the 1st term s.t.

$$\text{tr}(\frac{\partial C}{\partial X} C^T + C \frac{\partial C^T}{\partial X}),$$

then

$$= \frac{\partial(CC^T)}{\partial X} = \frac{\partial I}{\partial X} = 0 \quad \square$$